thys/ConcurrentIMP/CIMP.thy
@@ -16,7 +16,7 @@ imports
   CIMP_vcg
   "HOL-Library.Sublist"
 keywords
-  "locset_definition" :: thy_defn
+  "inv_definition" "locset_definition" :: thy_defn
 begin
 
 text\<open>
@@ -27,6 +27,7 @@ of use.
 \<close>
 
 named_theorems com "Command definitions"
+named_theorems inv "Location-sensitive invariant definitions"
 named_theorems loc "Location set membership cache"
 
 ML\<open>
@@ -35,7 +36,10 @@ signature CIMP =
 sig
     val com_locs_fold : (term -> 'b -> 'b) -> 'b -> term -> 'b
     val com_locs_map : (term -> 'b) -> term -> 'b list
-    val locset : thm -> local_theory -> local_theory
+    val com_locs_fold_no_response : (term -> 'b -> 'b) -> 'b -> term -> 'b
+    val com_locs_map_no_response : (term -> 'b) -> term -> 'b list
+    val def_inv : thm -> local_theory -> local_theory
+    val def_locset : thm -> local_theory -> local_theory
 end;
 
 structure Cimp : CIMP =
@@ -54,6 +58,19 @@ fun com_locs_fold f x (Const (@{const_name Request}, _) $ l $ _ $ _ )    = f l x
 
 fun com_locs_map f com = com_locs_fold (fn l => fn acc => f l :: acc) [] com
 
+fun com_locs_fold_no_response f x (Const (@{const_name Request}, _) $ l $ _ $ _ )    = f l x
+  | com_locs_fold_no_response _ x (Const (@{const_name Response}, _) $ _ $ _)        = x (* can often ignore \<open>Response\<close> *)
+  | com_locs_fold_no_response f x (Const (@{const_name LocalOp}, _) $ l $ _)         = f l x
+  | com_locs_fold_no_response f x (Const (@{const_name Cond1}, _) $ l $ _ $ c)       = com_locs_fold_no_response f (f l x) c
+  | com_locs_fold_no_response f x (Const (@{const_name Cond2}, _) $ l $ _ $ c1 $ c2) = com_locs_fold_no_response f (com_locs_fold_no_response f (f l x) c1) c2
+  | com_locs_fold_no_response f x (Const (@{const_name Loop}, _) $ c)                = com_locs_fold_no_response f x c
+  | com_locs_fold_no_response f x (Const (@{const_name While}, _) $ l $ _ $ c)       = com_locs_fold_no_response f (f l x) c
+  | com_locs_fold_no_response f x (Const (@{const_name Seq}, _) $ c1 $ c2)           = com_locs_fold_no_response f (com_locs_fold_no_response f x c1) c2
+  | com_locs_fold_no_response f x (Const (@{const_name Choose}, _) $ c1 $ c2)        = com_locs_fold_no_response f (com_locs_fold_no_response f x c1) c2
+  | com_locs_fold_no_response _ x _ = x;
+
+fun com_locs_map_no_response f com = com_locs_fold_no_response (fn l => fn acc => f l :: acc) [] com
+
 (* Cache location set membership facts.
 
 Decide membership in the given set for each label in the CIMP programs
@@ -61,42 +78,56 @@ in the Named_Theorems "com".
 
 If the label set and com types differ, we probably get a nasty error.
 
-No need to consider locations of @{const "Response"}s; could tweak
-@{text "com_locs_fold"} to reflect this.
-
 *)
 
-fun locset thm ctxt =
+fun def_locset thm ctxt =
   let
-    val set_name = thm |> Thm.cprop_of |> Thm.dest_equals |> fst |> Thm.term_of (* FIXME how do we handle HOL (=) as well? maybe rule_format? *)
+    val set_name = thm
+                   |> Local_Defs.meta_rewrite_rule ctxt (* handle `=` or `\<equiv>` *)
+                   |> Thm.cprop_of |> Thm.dest_equals |> fst |> Thm.term_of
     val set_typ = set_name |> type_of
     val elt_typ = case set_typ of Type ("Set.set", [t]) => t | _ => raise Fail "thm should define a set"
-    val set_name_str = case set_name of Const (c, _) => c | Free (c, _) => c | _ => raise Fail "FIXME not a constant XXX" (* FIXME `definition` spits out a thm with a Free in it *)
-    val thm_name = set_name_str |> Long_Name.base_name |> (fn def => def ^ "_membs")
+    val set_name_str = case set_name of Const (c, _) => c | Free (c, _) => c | _ => error ("Not an equation of the form x = set: " ^ Thm.string_of_thm ctxt thm)
+    val thm_name = Binding.qualify true set_name_str (Binding.name "memb")
     fun mk_memb l = Thm.cterm_of ctxt (Const (@{const_name "Set.member"}, elt_typ --> set_typ --> @{typ "bool"}) $ l $ set_name)
     val rewrite_tac = Simplifier.rewrite (ctxt addsimps ([thm] @ Named_Theorems.get ctxt @{named_theorems "loc"})) (* probably want the ambient simpset + some stuff *)
     val coms = Named_Theorems.get ctxt @{named_theorems "com"} |> map (Thm.cprop_of #> Thm.dest_equals #> snd #> Thm.term_of)
     val attrs = [(* Attrib.internal (K (Clasimp.iff_add)), *) Attrib.internal (K (Named_Theorems.add @{named_theorems "loc"}))]
 (* Parallel *)
-    fun mk_thms coms = Par_List.map rewrite_tac (maps (com_locs_map mk_memb) coms)
+    fun mk_thms coms = Par_List.map rewrite_tac (maps (com_locs_map_no_response mk_memb) coms)
 (* Sequential *)
 (*    fun mk_thms coms = List.foldl (fn (c, thms) => com_locs_fold (fn l => fn thms => rewrite_tac (mk_memb l) :: thms) thms c) [] coms *)
   in
     ctxt
-    |> (Local_Theory.note ((Binding.name thm_name, attrs), mk_thms coms) #>> snd)
+    |> Local_Theory.note ((thm_name, attrs), mk_thms coms)
+    |> snd
+  end;
+
+(* FIXME later need to rewrite using interned labels (fold defs). *)
+fun def_inv thm ctxt : local_theory =
+  let
+    val attrs = [Attrib.internal (K (Named_Theorems.add @{named_theorems "inv"}))]
+  in
+    ctxt
+    |> Local_Theory.note ((Binding.empty, attrs), [thm])
     |> snd
   end;
 
 end;
 
-(* `definition` + `locset` *)
+val _ =
+  Outer_Syntax.local_theory' \<^command_keyword>\<open>inv_definition\<close> "constant definition for invariants"
+    (Scan.option Parse_Spec.constdecl -- (Parse_Spec.opt_thm_name ":" -- Parse.prop) --
+      Parse_Spec.if_assumes -- Parse.for_fixes >> (fn (((decl, spec), prems), params) => fn b => fn lthy =>
+        Specification.definition_cmd decl params prems spec b lthy
+        |> (fn ((_, (_, thm)), lthy) => (thm, lthy)) |> uncurry Cimp.def_inv));
+
 val _ =
   Outer_Syntax.local_theory' \<^command_keyword>\<open>locset_definition\<close> "constant definition for sets of locations"
     (Scan.option Parse_Spec.constdecl -- (Parse_Spec.opt_thm_name ":" -- Parse.prop) --
       Parse_Spec.if_assumes -- Parse.for_fixes >> (fn (((decl, spec), prems), params) => fn b => fn lthy =>
         Specification.definition_cmd decl params prems spec b lthy
-        |> (fn ((_, (_, thm)), lthy) => (thm, lthy)) |> uncurry Cimp.locset));
-
+        |> (fn ((_, (_, thm)), lthy) => (thm, lthy)) |> uncurry Cimp.def_locset));
 \<close>
 
 end
