thys/ConcurrentGC/Tactics.thy
@@ -83,7 +83,6 @@ is the use of Isabelle's parallelism to greatly reduce system latency.
 
 subsection\<open>Tactics\<close>
 
-named_theorems inv "Location-sensitive invariant definitions"
 named_theorems nie "Non-interference elimination rules"
 
 text\<open>
@@ -247,6 +246,7 @@ fun vcg_jackhammer_gen_tac terminal_tac ctxt =
              THEN' asm_full_simp_tac (ss_only (@{thms loc_simps} @ Named_Theorems.get ctxt @{named_theorems loc}) ctxt)
              THEN_ALL_NEW (TRY o REPEAT_ALL_NEW (Rule_Insts.thin_tac ctxt "True" [])) (* FIXME weird, must be a standard way to do this. Leaving them in can cause simp to diverge ?? *)
              THEN_ALL_NEW clarsimp_tac (ctxt addsimps (Named_Theorems.get ctxt @{named_theorems loc} @ @{thms atS_simps})) (* FIXME smelly *)
+             THEN_ALL_NEW Rule_Insts.thin_tac ctxt "AT _ = _" [] (* FIXME discard \<open>AT s = s'(funupd)\<close> fact *)
              THEN_ALL_NEW TRY o terminal_tac ctxt)))
 
 val _ =
@@ -275,6 +275,7 @@ fun vcg_ni_tac ctxt =
       THEN_ALL_NEW (TRY o REPEAT_ALL_NEW (Tactic.ematch_tac ctxt @{thms thin_locs} THEN' REPEAT1 o assume_tac ctxt))
       THEN_ALL_NEW asm_full_simp_tac (ss_only (@{thms loc_simps} @ Named_Theorems.get ctxt @{named_theorems loc}) ctxt)
       THEN_ALL_NEW (TRY o REPEAT_ALL_NEW (Rule_Insts.thin_tac ctxt "True" [])) (* FIXME weird, must be a standard way to do this. Leaving them in can cause simp to diverge ?? *)
+(*      THEN_ALL_NEW Rule_Insts.thin_tac ctxt "AT _ = _" [] (* FIXME discard \<open>AT s = s'(funupd)\<close> fact *) doesn't work when processes communicate! see gc_sweep_loop_invL *)
       THEN_ALL_NEW clarsimp_tac ctxt))
 
 fun vcg_nihe_tac ctxt =
